One admit left

examples/br93.ec
@@ -10,8 +10,6 @@ require import Real.
 require import Pair.
 require import Word.
 
-
-
 op k : int. (* size of message *)
 op l : int. (* size of randmness *)
 op n : int. (* size of cipher *)
@@ -38,33 +36,31 @@ op uniform : plaintext distr = Plaintext.Dword.dword.
 op uniform_rand : randomness distr = Randomness.Dword.dword.
 
 clone RandOrcl as RandOrcl_BR with 
-  type from = randomness, 
-  type to = plaintext,
-  op dsample = uniform,
-  op qO = qH,
-  op default = Plaintext.zeros.
+type from = randomness, 
+type to = plaintext,
+op dsample = uniform,
+op qO = qH,
+op default = Plaintext.zeros.
 
 import RandOrcl_BR.
 import ROM.
 
 module type Scheme(RO : Oracle) = {
-   fun init(): unit 
-   fun kg() : (pkey * skey)
-   fun enc(pk:pkey, m:plaintext): ciphertext 
-  }.
+ fun init(): unit 
+ fun kg() : (pkey * skey)
+ fun enc(pk:pkey, m:plaintext): ciphertext 
+}.
 
 module type Adv(ARO : Oracle)  = {
  fun a1 (p : pkey) : (plaintext * plaintext) {ARO.o}
  fun a2 (c : ciphertext) : bool {ARO.o}
 }.
 
-
-
 module CPA(S : Scheme, A_ : Adv) = {
  module ARO = ARO(RO)
  module A = A_(ARO)
  module SO = S(RO)
- fun main(): bool = {
+  fun main(): bool = {
   var pk:pkey;
   var sk:skey;
   var m0 : plaintext;
@@ -83,27 +79,25 @@ module CPA(S : Scheme, A_ : Adv) = {
  } 
 }.
 
-
-
 op (||) (x : randomness, y : plaintext) : ciphertext =
-Ciphertext.from_array ((Randomness.to_array x) || (Plaintext.to_array y)).
+ Ciphertext.from_array ((Randomness.to_array x) || (Plaintext.to_array y)).
 
 module BR(R : Oracle) : Scheme(R) = {
  var r : randomness
+ 
  fun init() : unit = {
   r = $uniform_rand; 
  }
-
-   fun kg():(pkey * skey) = {
-   var pk, sk:(pkey * skey);
+ fun kg():(pkey * skey) = {
+  var pk, sk:(pkey * skey);
   (pk,sk) = $keypairs;
-   return (pk,sk);
+  return (pk,sk);
  }
  
-   fun enc(pk:pkey, m:plaintext): ciphertext = {
-   var h : plaintext;
-   h  = R.o(r);
-   return ((f pk r) ||  Plaintext.(^^) m h);
+ fun enc(pk:pkey, m:plaintext): ciphertext = {
+  var h : plaintext;
+  h  = R.o(r);
+  return ((f pk r) ||  Plaintext.(^^) m h);
  }
 }.
 
@@ -116,16 +110,16 @@ module BR2(R : Oracle) : Scheme(R) = {
   r = $uniform_rand; 
  }
 
-   fun kg():(pkey * skey) = {
-   var pk, sk:(pkey * skey);
+ fun kg():(pkey * skey) = {
+  var pk, sk:(pkey * skey);
   (pk,sk) = $keypairs;
-   return (pk,sk);
+  return (pk,sk);
  }
  
-   fun enc(pk:pkey, m:plaintext): ciphertext = {
-   var h : plaintext;
-   h = $uniform; 
-   return ((f pk r) ||  Plaintext.(^^) m h);
+ fun enc(pk:pkey, m:plaintext): ciphertext = {
+  var h : plaintext;
+  h = $uniform; 
+  return ((f pk r) ||  Plaintext.(^^) m h);
  }
 }.
 
@@ -141,12 +135,13 @@ lemma eq_except_dom2 : forall(x, y : 'a, m1, m2 : ('a,'b) map),
 
 lemma eq1_enc :
  equiv [ BR(RO).enc ~ BR2(RO).enc : 
-pk{1} = pk{2} /\ RO.m{1} = RO.m{2} /\ m{1} = m{2} /\ BR.r{1} = BR2.r{2} /\
+ pk{1} = pk{2} /\ RO.m{1} = RO.m{2} /\ m{1} = m{2} /\ BR.r{1} = BR2.r{2} /\
  !in_dom BR2.r{2} RO.m{2} ==>
-res{1} = res{2} /\ eq_except RO.m{1} RO.m{2} BR2.r{2}].
-fun.
-inline RO.o.
-wp;rnd;wp;skip;progress(try trivial).
+ res{1} = res{2} /\ eq_except RO.m{1} RO.m{2} BR2.r{2}].
+proof.
+ fun.
+ inline RO.o.
+ wp;rnd;wp;skip;progress(try trivial).
 save.
 
 lemma eq1 : forall (A <: Adv {BR,BR2,CPA,RO,ARO}), 
@@ -165,94 +160,122 @@ proof.
  (glob A){1} = (glob A){2} /\ c{1} = c{2})
 ((!mem BR2.r ARO.log){2} => res{1} = res{2}).
  fun (mem BR2.r ARO.log) 
-(ARO.log{1} = ARO.log{2} /\ eq_except RO.m{1} RO.m{2} BR2.r{2}).
+ (ARO.log{1} = ARO.log{2} /\ eq_except RO.m{1} RO.m{2} BR2.r{2}).
 progress(try trivial).
 progress(try trivial).
 assumption.
  fun.
  if;[trivial| |wp;skip;trivial].
  inline RO.o;wp;rnd;wp;skip;progress(try trivial).
- admit.
- admit.
-(* don't know how to use the spec I proved already *)
-(* call (pk{1} = pk{2} /\ RO.m{1} = RO.m{2} /\ m{1} = m{2} /\  *)
-(*      BR.r{1} = BR2.r{2} /\ !in_dom BR2.r{2} RO.m{2}) *)
-(*      (res{1} = res{2} /\ eq_except RO.m{1} RO.m{2} BR2.r{2}). *)
+ intros &m H. fun. 
+ seq 0: (3 = 3). (* fix this *)
+ skip;trivial.
+ if.
+ inline RO.o.
+ wp.
+ rnd 1%r cPtrue;wp;skip;progress(trivial).
+ wp;skip;progress(trivial).
 
-inline CPA(BR,A).SO.enc CPA(BR2,A).SO.enc RO.o.
-wp;rnd;wp;rnd.
+ intros &m. fun. 
+ if.
+ inline RO.o.
+ wp.
+ rnd 1%r cPtrue;wp;skip;progress(trivial).
+ wp;skip;progress(trivial).
+ (* don't know how to use the spec I proved already *)
+ (* call (pk{1} = pk{2} /\ RO.m{1} = RO.m{2} /\ m{1} = m{2} /\  *)
+ (*      BR.r{1} = BR2.r{2} /\ !in_dom BR2.r{2} RO.m{2}) *)
+ (*      (res{1} = res{2} /\ eq_except RO.m{1} RO.m{2} BR2.r{2}). *)
+
+ inline CPA(BR,A).SO.enc CPA(BR2,A).SO.enc RO.o.
+ wp;rnd;wp;rnd.
 call (p{1} = p{2} /\ (glob A){1} = (glob A){2} /\
  ARO.log{1} = ARO.log{2} /\ 
-RO.m{1} = RO.m{2} /\ 
-(forall (x : randomness), mem x ARO.log{2} <=> in_dom x RO.m{2}))
+ RO.m{1} = RO.m{2} /\ 
+ (forall (x : randomness), mem x ARO.log{2} <=> in_dom x RO.m{2}))
 (res{1} = res{2} /\ (glob A){1} = (glob A){2} /\
  ARO.log{1} = ARO.log{2} /\
-RO.m{1} = RO.m{2} /\
-(forall (x : randomness), mem x ARO.log{2} <=> in_dom x RO.m{2})).
-fun ( ARO.log{1} = ARO.log{2} /\
-RO.m{1} = RO.m{2} /\ 
-(forall (x : randomness), mem x ARO.log{2} <=> in_dom x RO.m{2}));try trivial.
-fun.
-if;[trivial| |wp;skip;trivial].
-inline RO.o;wp;rnd;wp;skip;progress(try trivial).
- inline CPA(BR,A).SO.kg CPA(BR2,A).SO.kg.
- wp;rnd.
-inline CPA(BR,A).ARO.init CPA(BR,A).SO.init RO.init
-       CPA(BR2,A).ARO.init CPA(BR2,A).SO.init RO.init.
-rnd;wp;skip;progress(try trivial).
+ RO.m{1} = RO.m{2} /\
+ (forall (x : randomness), mem x ARO.log{2} <=> in_dom x RO.m{2})).
+  fun ( ARO.log{1} = ARO.log{2} /\
+  RO.m{1} = RO.m{2} /\ 
+ (forall (x : randomness), mem x ARO.log{2} <=> in_dom x RO.m{2}));try trivial.
+  fun.
+  if;[trivial| |wp;skip;trivial].
+  inline RO.o;wp;rnd;wp;skip;progress(try trivial).
+  inline CPA(BR,A).SO.kg CPA(BR2,A).SO.kg.
+  wp;rnd.
+  inline CPA(BR,A).ARO.init CPA(BR,A).SO.init RO.init
+  CPA(BR2,A).ARO.init CPA(BR2,A).SO.init RO.init.
+  rnd;wp;skip;progress(try trivial).
 save.
 
 
 lemma prob1_1 :
-forall (A <: Adv {BR,BR2,CPA,RO,ARO}),
+ forall (A <: Adv {BR,BR2,CPA,RO,ARO}),
 (forall (O <: Oracle),
  bd_hoare[ O.o : true ==> true] = 1%r =>
  bd_hoare[ A(O).a2 : true ==> true] = 1%r) =>
-forall &m ,
+ forall &m ,
 Pr[CPA(BR,A).main() @ &m: res] <=
-Pr[CPA(BR2,A).main() @ &m : res || mem BR2.r ARO.log].
+Pr[CPA(BR2,A).main() @ &m : res \/ mem BR2.r ARO.log].
 proof.
-intros A Hlossless &m.
-equiv_deno (_ : (glob A){1} = (glob A){2} ==>
-  !(mem BR2.r ARO.log){2} => res{1} = res{2}).
-apply (eq1(<:A) _).
-assumption.
-trivial.
-trivial.
+ intros A Hlossless &m.
+ equiv_deno (_ : (glob A){1} = (glob A){2} ==>
+ !(mem BR2.r ARO.log){2} => res{1} = res{2}).
+ apply (eq1(<:A) _).
+ assumption.
+ trivial.
+ trivial.
 save.
 
 
 lemma prob1_2 :
-forall (A <: Adv {BR,BR2,CPA,RO,ARO}),
-forall &m,
-Pr[CPA(BR2,A).main() @ &m : res || mem BR2.r ARO.log] <=
+ forall (A <: Adv {BR,BR2,CPA,RO,ARO}),
+ forall &m,
+Pr[CPA(BR2,A).main() @ &m : res \/ mem BR2.r ARO.log] <=
 Pr[CPA(BR2,A).main() @ &m : res ] + 
 Pr[CPA(BR2,A).main() @ &m :  mem BR2.r ARO.log].
 proof.
-admit. 
+intros A &m.
+cut H:
+(Pr[CPA(BR2,A).main() @ &m : res \/ mem BR2.r ARO.log] =
+ Pr[CPA(BR2,A).main() @ &m : res] +  Pr[CPA(BR2,A).main() @ &m : mem BR2.r ARO.log] -
+ Pr[CPA(BR2,A).main() @ &m : res /\ mem BR2.r ARO.log]).
+pr_or;trivial.
+rewrite H.
+cut aux : (forall(a, b, c: real),0%r <= c => Real.(+) a b - c <= a + b).
+trivial.
+apply (aux (Pr[CPA(BR2,A).main() @ &m : res])
+           (Pr[CPA(BR2,A).main() @ &m : mem BR2.r ARO.log])
+           (Pr[CPA(BR2,A).main() @ &m : res /\ mem BR2.r ARO.log]) _).
+bdhoare_deno (_ : true ==> res /\ mem BR2.r ARO.log).
+fun;pr_bounded;trivial.
+trivial.
+trivial.
 save.
 
 lemma real_le_trans : forall(a, b, c : real),  
-      Real.(<=) a b => Real.(<=) b  c => a <= c by [].
+ Real.(<=) a b => Real.(<=) b  c => a <= c by [].
 
 lemma prob1_3 :
-forall (A <: Adv {BR,BR2,CPA,RO,ARO}),
+ forall (A <: Adv {BR,BR2,CPA,RO,ARO}),
 (forall (O <: Oracle),
  bd_hoare[ O.o : true ==> true] = 1%r =>
  bd_hoare[ A(O).a2 : true ==> true] = 1%r) =>
-forall &m,
+ forall &m,
 Pr[CPA(BR,A).main() @ &m: res] <=
 Pr[CPA(BR2,A).main() @ &m : res ] + 
 Pr[CPA(BR2,A).main() @ &m :  mem BR2.r ARO.log].
 proof.
-intros A Hlossless &m.
-apply (real_le_trans 
-           Pr[CPA(BR,A).main() @ &m: res] 
-           Pr[CPA(BR2,A).main() @ &m : res || mem BR2.r ARO.log]
-           (Pr[CPA(BR2,A).main() @ &m : res] + 
-              Pr[CPA(BR2,A).main() @ &m : mem BR2.r ARO.log]) _ _).
-apply (prob1_1 (<:A) _ &m );try trivial;assumption.
-apply (prob1_2 (<:A) &m).
+ intros A Hlossless &m.
+ apply (real_le_trans 
+ Pr[CPA(BR,A).main() @ &m: res] 
+ Pr[CPA(BR2,A).main() @ &m : res \/ mem BR2.r ARO.log]
+ (Pr[CPA(BR2,A).main() @ &m : res] + 
+  Pr[CPA(BR2,A).main() @ &m : mem BR2.r ARO.log]) _ _).
+   apply (prob1_1 (<:A) _ &m );try trivial;assumption.
+   apply (prob1_2 (<:A) &m).
 save.
 
 
@@ -270,18 +293,18 @@ module BR3(R : Oracle) : Scheme(R) = {
  
    fun enc(pk:pkey, m:plaintext): ciphertext = {
    var h : plaintext;
-   h = $uniform; 
+  h = $uniform; 
    return ((f pk r) ||  h);
  }
 }.
 
 lemma eq2_enc :
  equiv [ BR2(RO).enc ~ BR3(RO).enc : 
-pk{1} = pk{2} /\ RO.m{1} = RO.m{2} /\ m{1} = m{2} /\ BR2.r{1} = BR3.r{2} ==>
-res{1} = res{2} /\ RO.m{1} = RO.m{2}].
-fun.
-rnd (lambda v, Plaintext.(^^) m{2} v)(lambda v, Plaintext.(^^) m{2} v);skip.
-progress (trivial).
+ pk{1} = pk{2} /\ RO.m{1} = RO.m{2} /\ m{1} = m{2} /\ BR2.r{1} = BR3.r{2} ==>
+ res{1} = res{2} /\ RO.m{1} = RO.m{2}].
+ fun.
+ rnd (lambda v, Plaintext.(^^) m{2} v)(lambda v, Plaintext.(^^) m{2} v);skip.
+ progress (trivial).
 save.
 
 lemma eq2 : forall (A <: Adv {BR2,BR3,CPA,RO,ARO}), 
@@ -289,89 +312,89 @@ lemma eq2 : forall (A <: Adv {BR2,BR3,CPA,RO,ARO}),
  bd_hoare[ O.o : true ==> true] = 1%r =>
  bd_hoare[ A(O).a2 : true ==> true] = 1%r) =>
  equiv [ CPA(BR2,A).main ~ CPA(BR3,A).main : 
-(glob A){1} = (glob A){2} ==>
+ (glob A){1} = (glob A){2} ==>
  res{1} = res{2} /\ 
-ARO.log{1} = ARO.log{2} /\ BR2.r{1} = BR3.r{2}].
+  ARO.log{1} = ARO.log{2} /\ BR2.r{1} = BR3.r{2}].
 proof.
-intros A Hlossless.
-fun.
-call (ARO.log{1} = ARO.log{2} /\ RO.m{1} = RO.m{2} /\ 
-      c{1} = c{2} /\ (glob A){1} = (glob A){2})
+ intros A Hlossless.
+ fun.
+ call (ARO.log{1} = ARO.log{2} /\ RO.m{1} = RO.m{2} /\ 
+ c{1} = c{2} /\ (glob A){1} = (glob A){2})
 (ARO.log{1} = ARO.log{2} /\ RO.m{1} = RO.m{2} /\ 
  res{1} = res{2}).
-fun ((ARO.log{1} = ARO.log{2} /\ RO.m{1} = RO.m{2})).
-trivial.
-trivial.
-fun.
-if;[trivial| |].
-inline RO.o.
-wp;rnd;wp;skip;trivial.
-wp;skip;trivial.
-(* cannot use spec eq2_enc *)
-inline CPA(BR2, A).SO.enc CPA(BR3, A).SO.enc.
-wp.
-rnd (lambda v,Plaintext.(^^) m{2}  v)(lambda v,Plaintext.(^^) m{2}  v).
-simplify.
-wp;rnd.
-call (ARO.log{1} = ARO.log{2} /\ RO.m{1} = RO.m{2} /\ 
-      p{1} = p{2} /\ (glob A){1} = (glob A){2})
+ fun ((ARO.log{1} = ARO.log{2} /\ RO.m{1} = RO.m{2})).
+ trivial.
+ trivial.
+ fun.
+ if;[trivial| |].
+ inline RO.o.
+ wp;rnd;wp;skip;trivial.
+ wp;skip;trivial.
+ (* cannot use spec eq2_enc *)
+ inline CPA(BR2, A).SO.enc CPA(BR3, A).SO.enc.
+ wp.
+ rnd (lambda v,Plaintext.(^^) m{2}  v)(lambda v,Plaintext.(^^) m{2}  v).
+ simplify.
+ wp;rnd.
+ call (ARO.log{1} = ARO.log{2} /\ RO.m{1} = RO.m{2} /\ 
+ p{1} = p{2} /\ (glob A){1} = (glob A){2})
 (ARO.log{1} = ARO.log{2} /\ RO.m{1} = RO.m{2} /\ 
  res{1} = res{2}/\ (glob A){1} = (glob A){2}).
-fun ((ARO.log{1} = ARO.log{2} /\ RO.m{1} = RO.m{2})).
-trivial.
-trivial.
-fun.
-if;[trivial| |wp;skip;trivial].
-inline RO.o.
-wp;rnd;wp;skip;trivial.
+ fun ((ARO.log{1} = ARO.log{2} /\ RO.m{1} = RO.m{2})).
+ trivial.
+ trivial.
+ fun.
+ if;[trivial| |wp;skip;trivial].
+ inline RO.o.
+ wp;rnd;wp;skip;trivial.
 
-inline CPA(BR2, A).SO.init CPA(BR2, A).SO.kg CPA(BR2, A).ARO.init RO.init 
-       CPA(BR3, A).SO.init CPA(BR3, A).SO.kg CPA(BR3, A).ARO.init.
-wp;rnd;wp;rnd;wp;skip;progress (try trivial).
+ inline CPA(BR2, A).SO.init CPA(BR2, A).SO.kg CPA(BR2, A).ARO.init RO.init 
+ CPA(BR3, A).SO.init CPA(BR3, A).SO.kg CPA(BR3, A).ARO.init.
+ wp;rnd;wp;rnd;wp;skip;progress (try trivial).
 save.
 
 
 lemma prob2_1 : 
-forall (A <: Adv {BR2,BR3,CPA,RO,ARO}), 
+ forall (A <: Adv {BR2,BR3,CPA,RO,ARO}), 
 (forall (O <: Oracle),
  bd_hoare[ O.o : true ==> true] = 1%r =>
  bd_hoare[ A(O).a2 : true ==> true] = 1%r) =>
-forall &m,
+ forall &m,
 Pr[CPA(BR2,A).main() @ &m: res] =
 Pr[CPA(BR3,A).main() @ &m : res].
 proof.
-intros A Hlossless &m.
-equiv_deno (_ : (glob A){1} = (glob A){2} ==> 
-                 res{1} = res{2} /\ ARO.log{1} = ARO.log{2} /\ BR2.r{1} = BR3.r{2}).
-apply (eq2(<:A) _).
-assumption.
-trivial.
-trivial.
+ intros A Hlossless &m.
+ equiv_deno (_ : (glob A){1} = (glob A){2} ==> 
+ res{1} = res{2} /\ ARO.log{1} = ARO.log{2} /\ BR2.r{1} = BR3.r{2}).
+ apply (eq2(<:A) _).
+ assumption.
+ trivial.
+ trivial.
 save.
 
 lemma prob2_2 : 
-forall (A <: Adv {BR2,BR3,CPA,RO,ARO}), 
+ forall (A <: Adv {BR2,BR3,CPA,RO,ARO}), 
 (forall (O <: Oracle),
  bd_hoare[ O.o : true ==> true] = 1%r =>
  bd_hoare[ A(O).a2 : true ==> true] = 1%r) =>
-forall &m,
+ forall &m,
 Pr[CPA(BR2,A).main() @ &m: mem BR2.r ARO.log] =
 Pr[CPA(BR3,A).main() @ &m : mem BR3.r ARO.log].
 proof.
-intros A Hlossless &m.
-equiv_deno (_ : (glob A){1} = (glob A){2} ==> 
-                 res{1} = res{2} /\ ARO.log{1} = ARO.log{2} /\ BR2.r{1} = BR3.r{2}).
-apply (eq2(<:A) _).
-assumption.
-trivial.
-trivial.
+ intros A Hlossless &m.
+ equiv_deno (_ : (glob A){1} = (glob A){2} ==> 
+ res{1} = res{2} /\ ARO.log{1} = ARO.log{2} /\ BR2.r{1} = BR3.r{2}).
+ apply (eq2(<:A) _).
+ assumption.
+ trivial.
+ trivial.
 save.
 
 module CPA2(S : Scheme, A_ : Adv) = {
  module ARO = ARO(RO)
  module A = A_(ARO)
  module SO = S(RO)
- fun main(): bool = {
+  fun main(): bool = {
   var pk:pkey;
   var sk:skey;
   var m0 : plaintext;
@@ -395,98 +418,102 @@ lemma eq3 : forall (A <: Adv {BR3,CPA,CPA2,RO,ARO}),
  bd_hoare[ O.o : true ==> true] = 1%r =>
  bd_hoare[ A(O).a2 : true ==> true] = 1%r) =>
  equiv [ CPA(BR3,A).main ~ CPA2(BR3,A).main : 
-(glob A){1} = (glob A){2} ==>
+ (glob A){1} = (glob A){2} ==>
  res{1} = res{2} /\ 
-ARO.log{1} = ARO.log{2} /\ BR3.r{1} = BR3.r{2}].
+  ARO.log{1} = ARO.log{2} /\ BR3.r{1} = BR3.r{2}].
 proof.
-intros A Hlossless.
-fun.
-swap{2} -1.
-call (ARO.log{1} = ARO.log{2} /\ RO.m{1} = RO.m{2} /\ 
-      c{1} = c{2} /\ (glob A){1} = (glob A){2})
+ intros A Hlossless.
+ fun.
+ swap{2} -1.
+ call (ARO.log{1} = ARO.log{2} /\ RO.m{1} = RO.m{2} /\ 
+ c{1} = c{2} /\ (glob A){1} = (glob A){2})
 (ARO.log{1} = ARO.log{2} /\ RO.m{1} = RO.m{2} /\ 
  res{1} = res{2}).
-fun ((ARO.log{1} = ARO.log{2} /\ RO.m{1} = RO.m{2})).
-trivial.
-trivial.
-fun.
-if;[trivial| |].
-inline RO.o.
-wp;rnd;wp;skip;trivial.
-wp;skip;trivial.
-(* cannot use spec eq2_enc *)
-inline CPA(BR3, A).SO.enc CPA2(BR3, A).SO.enc.
-wp.
-swap{2} -2.
-wp;rnd;wp;rnd;wp.
-call (ARO.log{1} = ARO.log{2} /\ RO.m{1} = RO.m{2} /\ 
-      p{1} = p{2} /\ (glob A){1} = (glob A){2})
+ fun ((ARO.log{1} = ARO.log{2} /\ RO.m{1} = RO.m{2})).
+ trivial.
+ trivial.
+ fun.
+ if;[trivial| |].
+ inline RO.o.
+ wp;rnd;wp;skip;trivial.
+ wp;skip;trivial.
+ (* cannot use spec eq2_enc *)
+ inline CPA(BR3, A).SO.enc CPA2(BR3, A).SO.enc.
+ wp.
+ swap{2} -2.
+ wp;rnd;wp;rnd;wp.
+ call (ARO.log{1} = ARO.log{2} /\ RO.m{1} = RO.m{2} /\ 
+ p{1} = p{2} /\ (glob A){1} = (glob A){2})
 (ARO.log{1} = ARO.log{2} /\ RO.m{1} = RO.m{2} /\ 
  res{1} = res{2}/\ (glob A){1} = (glob A){2}).
-fun ((ARO.log{1} = ARO.log{2} /\ RO.m{1} = RO.m{2})).
-trivial.
-trivial.
-fun.
-if;[trivial| |wp;skip;trivial].
-inline RO.o.
-wp;rnd;wp;skip;trivial.
+ fun ((ARO.log{1} = ARO.log{2} /\ RO.m{1} = RO.m{2})).
+ trivial.
+ trivial.
+ fun.
+ if;[trivial| |wp;skip;trivial].
+ inline RO.o.
+ wp;rnd;wp;skip;trivial.
 
-inline CPA2(BR3, A).SO.init CPA2(BR3, A).SO.kg CPA2(BR3, A).ARO.init RO.init 
-       CPA(BR3, A).SO.init CPA(BR3, A).SO.kg CPA(BR3, A).ARO.init.
-wp;rnd;wp;rnd;wp;skip;progress (try trivial).
+ inline CPA2(BR3, A).SO.init CPA2(BR3, A).SO.kg CPA2(BR3, A).ARO.init RO.init 
+ CPA(BR3, A).SO.init CPA(BR3, A).SO.kg CPA(BR3, A).ARO.init.
+ wp;rnd;wp;rnd;wp;skip;progress (try trivial).
 save.
 
 lemma prob3_1 : 
-forall (A <: Adv {CPA2,BR3,CPA,RO,ARO}), 
+ forall (A <: Adv {CPA2,BR3,CPA,RO,ARO}), 
 (forall (O <: Oracle),
  bd_hoare[ O.o : true ==> true] = 1%r =>
  bd_hoare[ A(O).a2 : true ==> true] = 1%r) =>
-forall &m,
-  Pr[CPA2(BR3,A).main()  @ &m : res] = 1%r / 2%r.
+ forall &m,
+Pr[CPA2(BR3,A).main()  @ &m : res] = 1%r / 2%r.
 proof.
-intros A Hlossless.
-intros &m.
-cut H1 : (bd_hoare[CPA2(BR3,A).main : true ==> res] = (1%r / 2%r)).
-  fun; rnd (1%r / 2%r) (lambda b, b = b'); simplify.
+ intros A Hlossless.
+ intros &m.
+ cut H1 : (bd_hoare[CPA2(BR3,A).main : true ==> res] = (1%r / 2%r)).
+ fun; rnd (1%r / 2%r) (lambda b, b = b'); simplify.
  admit.
-  bdhoare_deno H1; trivial.
+ (* seq 5: (true).
+ inline CPA2(BR3,A).SO.enc.
+ wp. *)
+ 
+ bdhoare_deno H1; trivial.
 save.
 
 
 lemma prob3_2 : 
-forall (A <: Adv {BR3,CPA,CPA2,RO,ARO}), 
+ forall (A <: Adv {BR3,CPA,CPA2,RO,ARO}), 
 (forall (O <: Oracle),
  bd_hoare[ O.o : true ==> true] = 1%r =>
  bd_hoare[ A(O).a2 : true ==> true] = 1%r) =>
-forall &m, 
+ forall &m, 
 Pr[CPA(BR3,A).main() @ &m: res] =
 Pr[CPA2(BR3,A).main() @ &m : res].
 proof.
-intros A Hlossless &m.
-equiv_deno (_ : (glob A){1} = (glob A){2} ==> 
-                 res{1} = res{2} /\ ARO.log{1} = ARO.log{2} /\ BR3.r{1} = BR3.r{2}).
-apply (eq3(<:A) _).
-assumption.
-trivial.
-trivial.
+ intros A Hlossless &m.
+ equiv_deno (_ : (glob A){1} = (glob A){2} ==> 
+ res{1} = res{2} /\ ARO.log{1} = ARO.log{2} /\ BR3.r{1} = BR3.r{2}).
+ apply (eq3(<:A) _).
+ assumption.
+ trivial.
+ trivial.
 save.
 
 lemma prob3_3 : 
-forall (A <: Adv {BR3,CPA,CPA2,RO,ARO}), 
+ forall (A <: Adv {BR3,CPA,CPA2,RO,ARO}), 
 (forall (O <: Oracle),
  bd_hoare[ O.o : true ==> true] = 1%r =>
  bd_hoare[ A(O).a2 : true ==> true] = 1%r) =>
-forall &m,
+ forall &m,
 Pr[CPA(BR3,A).main() @ &m: mem BR3.r ARO.log] =
 Pr[CPA2(BR3,A).main() @ &m : mem BR3.r ARO.log].
 proof.
-intros A Hlossless &m.
-equiv_deno (_ : (glob A){1} = (glob A){2} ==> 
-                 res{1} = res{2} /\ ARO.log{1} = ARO.log{2} /\ BR3.r{1} = BR3.r{2}).
-apply (eq3(<:A) _).
-assumption.
-trivial.
-trivial.
+ intros A Hlossless &m.
+ equiv_deno (_ : (glob A){1} = (glob A){2} ==> 
+ res{1} = res{2} /\ ARO.log{1} = ARO.log{2} /\ BR3.r{1} = BR3.r{2}).
+ apply (eq3(<:A) _).
+ assumption.
+ trivial.
+ trivial.
 save.
 
 
@@ -511,7 +538,7 @@ module OW(I :Inverter) ={
 module BR_OW(A_ : Adv) : Inverter = {
  module ARO = ARO(RO)
  module A = A_(ARO)
- fun i(pk : pkey,y : randomness) : randomness ={
+  fun i(pk : pkey,y : randomness) : randomness ={
   var m0 : plaintext;
   var m1 : plaintext;
   var h : plaintext;
@@ -522,7 +549,7 @@ module BR_OW(A_ : Adv) : Inverter = {
   h = $uniform; 
   b  = A.a2(y || h);
   x = proj (Map.find (lambda p,f pk (Pair.fst p) = y) RO.m);
-  return (x);
+   return (x);
  }
 }.
 
@@ -531,94 +558,94 @@ lemma eq4 : forall (A <: Adv {BR3,CPA2,RO,ARO,BR_OW}),
  bd_hoare[ O.o : true ==> true] = 1%r =>
  bd_hoare[ A(O).a2 : true ==> true] = 1%r) =>
  equiv [ CPA2(BR3,A).main ~ OW(BR_OW(A)).main : 
-(glob A){1} = (glob A){2} ==> (mem BR3.r{1} ARO.log{1} => res{2})].
+ (glob A){1} = (glob A){2} ==> (mem BR3.r{1} ARO.log{1} => res{2})].
 proof.
-intros A Hlossless.
-fun.
-rnd{1}.
-inline  BR_OW(A).i.
-wp.
+ intros A Hlossless.
+ fun.
+ rnd{1}.
+ inline  BR_OW(A).i.
+ wp.
 call ((glob A){1} = (glob A){2} /\ c{1} = c{2} /\
-       RO.m{1} = RO.m{2} /\ ARO.log{1} = ARO.log{2})
+ RO.m{1} = RO.m{2} /\ ARO.log{1} = ARO.log{2})
 ((glob A){1} = (glob A){2} /\
-       RO.m{1} = RO.m{2} /\ ARO.log{1} = ARO.log{2} /\ res{1} = res{2}).
-fun (RO.m{1} = RO.m{2} /\ ARO.log{1} = ARO.log{2}).
-trivial.
-trivial.
-fun.
-if;[trivial|inline RO.o;wp;rnd |];wp;skip;progress(try trivial).
-inline CPA2(BR3,A).SO.enc.
-wp.
-rnd.
-wp.
+ RO.m{1} = RO.m{2} /\ ARO.log{1} = ARO.log{2} /\ res{1} = res{2}).
+ fun (RO.m{1} = RO.m{2} /\ ARO.log{1} = ARO.log{2}).
+ trivial.
+ trivial.
+ fun.
+ if;[trivial|inline RO.o;wp;rnd |];wp;skip;progress(try trivial).
+ inline CPA2(BR3,A).SO.enc.
+ wp.
+ rnd.
+ wp.
 call ((glob A){1} = (glob A){2} /\ p{1} = p{2} /\
-       RO.m{1} = RO.m{2} /\ ARO.log{1} = ARO.log{2})
+ RO.m{1} = RO.m{2} /\ ARO.log{1} = ARO.log{2})
 ((glob A){1} = (glob A){2} /\
-       RO.m{1} = RO.m{2} /\ ARO.log{1} = ARO.log{2} /\ res{1} = res{2}).
-fun (RO.m{1} = RO.m{2} /\ ARO.log{1} = ARO.log{2}).
-trivial.
-trivial.
-fun.
-if;[trivial|inline RO.o;wp;rnd |];wp;skip;progress(try trivial).
-inline CPA2(BR3, A).SO.init CPA2(BR3, A).ARO.init RO.init CPA2(BR3, A).SO.kg 
-BR_OW(A).ARO.init.
-wp;!2 rnd;wp;skip;progress(try trivial).
+ RO.m{1} = RO.m{2} /\ ARO.log{1} = ARO.log{2} /\ res{1} = res{2}).
+ fun (RO.m{1} = RO.m{2} /\ ARO.log{1} = ARO.log{2}).
+ trivial.
+ trivial.
+ fun.
+ if;[trivial|inline RO.o;wp;rnd |];wp;skip;progress(try trivial).
+ inline CPA2(BR3, A).SO.init CPA2(BR3, A).ARO.init RO.init CPA2(BR3, A).SO.kg 
+ BR_OW(A).ARO.init.
+ wp;!2 rnd;wp;skip;progress(try trivial).
 save.
 
 
 lemma Reduction (A <: Adv {CPA,CPA2, BR, BR2, BR3, OW, RO, ARO, BR_OW}) &m : 
-  (forall (O <: Oracle),
-   bd_hoare[ O.o : true ==> true] = 1%r =>
-   bd_hoare[ A(O).a2 : true ==> true] = 1%r) =>
-  Pr[CPA(BR,A).main() @ &m : res] <=
-  1%r / 2%r + Pr[OW(BR_OW(A)).main() @ &m : res].
-intros Hlossless.
-apply (real_le_trans 
-(Pr[CPA(BR, A).main() @ &m : res])
-(Pr[CPA(BR2,A).main() @ &m : res ] + 
-Pr[CPA(BR2,A).main() @ &m : mem BR2.r ARO.log])
-(1%r / 2%r + Pr[OW(BR_OW(A)).main() @ &m : res]) _ _).
-apply (prob1_3(<:A) _ &m).
-assumption.
-rewrite (prob2_1(<:A) _ &m).
-assumption.
-rewrite (prob2_2(<:A) _ &m).
-assumption.
-rewrite (prob3_2(<:A) _ &m).
-assumption.
-rewrite (prob3_3(<:A) _ &m).
-assumption.
-rewrite (prob3_1(<:A) _ &m).
-assumption.
-cut aux: (forall (a b c : real), b <= c => a + b <= a + c).
-trivial.
-apply (aux (1%r/2%r) (Pr[CPA2(BR3,A).main() @ &m : mem BR3.r ARO.log])
-      Pr[OW(BR_OW(A)).main() @ &m : res] _).
-equiv_deno (_ : (glob A){1} = (glob A){2} ==> 
-                 mem BR3.r{1} ARO.log{1} => res{2}).
-apply (eq4(<:A) _).
-assumption.
-trivial.
-trivial.
+(forall (O <: Oracle),
+ bd_hoare[ O.o : true ==> true] = 1%r =>
+ bd_hoare[ A(O).a2 : true ==> true] = 1%r) =>
+Pr[CPA(BR,A).main() @ &m : res] <=
+ 1%r / 2%r + Pr[OW(BR_OW(A)).main() @ &m : res].
+ intros Hlossless.
+ apply (real_le_trans 
+ (Pr[CPA(BR, A).main() @ &m : res])
+ (Pr[CPA(BR2,A).main() @ &m : res ] + 
+  Pr[CPA(BR2,A).main() @ &m : mem BR2.r ARO.log])
+ (1%r / 2%r + Pr[OW(BR_OW(A)).main() @ &m : res]) _ _).
+  apply (prob1_3(<:A) _ &m).
+  assumption.
+  rewrite (prob2_1(<:A) _ &m).
+  assumption.
+  rewrite (prob2_2(<:A) _ &m).
+  assumption.
+  rewrite (prob3_2(<:A) _ &m).
+  assumption.
+  rewrite (prob3_3(<:A) _ &m).
+  assumption.
+  rewrite (prob3_1(<:A) _ &m).
+  assumption.
+  cut aux: (forall (a b c : real), b <= c => a + b <= a + c).
+  trivial.
+  apply (aux (1%r/2%r) (Pr[CPA2(BR3,A).main() @ &m : mem BR3.r ARO.log])
+ Pr[OW(BR_OW(A)).main() @ &m : res] _).
+  equiv_deno (_ : (glob A){1} = (glob A){2} ==> 
+  mem BR3.r{1} ARO.log{1} => res{2}).
+  apply (eq4(<:A) _).
+  assumption.
+  trivial.
+  trivial.
 save.
 
 
 lemma Conclusion (A <: Adv {CPA,CPA2, BR, BR2, BR3, OW, RO, ARO, BR_OW}) &m :
-  (forall (O <: Oracle),
-   bd_hoare[ O.o : true ==> true] = 1%r =>
-   bd_hoare[ A(O).a2 : true ==> true] = 1%r) =>
-  exists (I<:Inverter), 
-    Pr[CPA(BR,A).main() @ &m : res] - 1%r / 2%r <= 
-    Pr[OW(BR_OW(A)).main() @ &m : res].
+(forall (O <: Oracle),
+ bd_hoare[ O.o : true ==> true] = 1%r =>
+ bd_hoare[ A(O).a2 : true ==> true] = 1%r) =>
+ exists (I<:Inverter), 
+Pr[CPA(BR,A).main() @ &m : res] - 1%r / 2%r <= 
+Pr[OW(BR_OW(A)).main() @ &m : res].
 proof.
-  intros H.
-  exists (<:BR_OW(A)).
-  cut aux : 
- (forall (x, y:real), x <= 1%r / 2%r + y => x - 1%r / 2%r  <= y). 
-  trivial.
-  apply (aux
-   Pr[CPA(BR,A).main() @ &m : res]
-   Pr[OW(BR_OW(A)).main() @ &m : res] _).
+ intros H.
+ exists (<:BR_OW(A)).
+ cut aux : 
+(forall (x, y:real), x <= 1%r / 2%r + y => x - 1%r / 2%r  <= y). 
+ trivial.
+ apply (aux
+ Pr[CPA(BR,A).main() @ &m : res]
+ Pr[OW(BR_OW(A)).main() @ &m : res] _).
   apply (Reduction (<:A) &m _).
   assumption.
 save.
